First attempt of constructing the comp program. This will be probably be complicated to verify, but it is what it is.

Loop/Basic.lean
@@ -22,6 +22,7 @@ Loop-computable is the same as primitive recursive.
 namespace Loop
 
 open Program
+open Mathlib (Vector)
 
 theorem loop_computable_cleanly_is_loop_computable : loop_computable_cleanly f → loop_computable f := by
   rename_i n
@@ -74,54 +75,53 @@ theorem get_is_loop_computable_cleanly (i : Fin n) : loop_computable_cleanly (fu
   intro v
   have : i + 1 - n = 0 := by exact Nat.sub_eq_zero_iff_le.2 i.isLt
   simp [init_state, highest_var, this, p, execution_from_state,
-    loop_inc_adds_value, value_at_cons_succ, value_at, Mathlib.Vector.get_eq_get]
-
--- theorem comp_is_loop_computable_cleanly (g : Fin n → VectNat m → Nat) :
---       loop_computable_cleanly f
---     → (∀ i, loop_computable_cleanly (g i))
---     → loop_computable_cleanly fun a => f (Mathlib.Vector.ofFn fun i => g i a) := by
---   sorry
+    loop_inc_adds_value, value_at_cons_succ, value_at, Vector.get_eq_get]
 
 section prec_is_loop_computable_cleanly_proof
 
-variable {n : Nat} {f : VectNat n → Nat} {g : VectNat (n + 2) → Nat} (f_h : cleanly_computes p_f f) (g_h : cleanly_computes p_g g)
+variable
+  {n : Nat}
+  {f : VectNat n → Nat}
+  {g : VectNat (n + 2) → Nat}
+  (f_h : cleanly_computes p_f f)
+  (g_h : cleanly_computes p_g g)
 
 -- Part I: construction of the program
 
-def offset (_ : cleanly_computes p_f f) (_ : cleanly_computes p_g g) : Nat :=  max (n + 2) (max (highest_var p_f) (highest_var p_g))
+def offset_pr (_ : cleanly_computes p_f f) (_ : cleanly_computes p_g g) : Nat :=  max (n + 2) (max (highest_var p_f) (highest_var p_g))
 
 -- Step 1: compute f of the last n inputs
 def prec_program_1 : Program :=
-  let offset := offset f_h g_h
-  let p_1_1 := store_X_1_to_X_succ_n (offset + 1) n
+  let offset_pr := offset_pr f_h g_h
+  let p_1_1 := store_X_1_to_X_succ_n (offset_pr + 1) n
   let p_1_2 := clear_X_j_to_X_n_plus_j 1 n
   let p_1_3 := match (generalizing := false) n with
     | 0 => p_f
-    | n + 1 => setup_X_j_to_X_n_plus_j (offset + 1) 1 n ++ p_f
+    | n + 1 => setup_X_j_to_X_n_plus_j (offset_pr + 1) 1 n ++ p_f
   p_1_1 ++ p_1_2 ++ p_1_3
 
 -- Step 2: compute g counter number of times, for each recursive step
 def prec_program_2 : Program :=
-  let offset := offset f_h g_h
+  let offset_pr := offset_pr f_h g_h
   let p_2_1 := X 2 += X 0
   let p_2_2 := CLEAR X 0
   let p_2_3 := p_g
   let p_2_4 := CLEAR X 2
   let p_2_5 := INC X 1
   let loop_inner := p_2_1 ++ p_2_2 ++ p_2_3 ++ p_2_4 ++ p_2_5
-  let p_loop := LOOP X (offset + 1) DO loop_inner END
+  let p_loop := LOOP X (offset_pr + 1) DO loop_inner END
   match (generalizing := false) n with
     | 0 => p_loop
-    | n + 1 => clear_X_j_to_X_n_plus_j 1 n ++ setup_X_j_to_X_n_plus_j (offset + 1) 3 n ++ p_loop
+    | n + 1 => clear_X_j_to_X_n_plus_j 1 n ++ setup_X_j_to_X_n_plus_j (offset_pr + 1) 3 n ++ p_loop
 
 -- Step 3: Clean up
 def prec_program_3 : Program :=
-  let offset := offset f_h g_h
+  let offset_pr := offset_pr f_h g_h
   let p_3_1 := match (generalizing := false) n with
     | 0 => CLEAR X 1
     | n + 1 => CLEAR X 1 ++ clear_X_j_to_X_n_plus_j 3 n
-  let p_3_2 := setup_X_j_to_X_n_plus_j offset 1 n
-  let p_3_3 := clear_Z_0_to_Z_n (offset + 1) n
+  let p_3_2 := setup_X_j_to_X_n_plus_j offset_pr 1 n
+  let p_3_3 := clear_Z_0_to_Z_n (offset_pr + 1) n
   p_3_1 ++ p_3_2 ++ p_3_3
 
 def prec_program : Program :=
@@ -132,7 +132,7 @@ def prec_program : Program :=
 
 -- Part II: calculate the highest variable of the program
 
-theorem prec_program_1_highest_var : highest_var (prec_program_1 f_h g_h) = offset f_h g_h + 1 + n := by
+theorem prec_program_1_highest_var : highest_var (prec_program_1 f_h g_h) = offset_pr f_h g_h + 1 + n := by
   simp [prec_program_1]
   repeat rewrite [highest_var_concat]
   rewrite [highest_var_store, highest_var_clear]
@@ -140,58 +140,58 @@ theorem prec_program_1_highest_var : highest_var (prec_program_1 f_h g_h) = offs
   cases n
   case zero =>
     simp_arith
-    have : highest_var p_f ≤ offset f_h g_h := by simp [offset]
+    have : highest_var p_f ≤ offset_pr f_h g_h := by simp [offset_pr ]
     exact Nat.le_trans this (Nat.le_add_right _ 1)
   case succ n =>
     rewrite [highest_var_concat, highest_var_setup]
-    have : max (n + 1 + 1) (offset f_h g_h + 1 + (n + 1)) = offset f_h g_h + 1 + (n + 1) := by simp_arith
+    have : max (n + 1 + 1) (offset_pr f_h g_h + 1 + (n + 1)) = offset_pr f_h g_h + 1 + (n + 1) := by simp_arith
     rewrite [this]
-    have : max (n + 1) (offset f_h g_h + 1 + n + 1) = offset f_h g_h + 1 + n + 1 := by simp_arith
+    have : max (n + 1) (offset_pr f_h g_h + 1 + n + 1) = offset_pr f_h g_h + 1 + n + 1 := by simp_arith
     rewrite [this]
-    have : max (offset f_h g_h + 1 + n + 1) (highest_var p_f) = offset f_h g_h + 1 + n + 1 := by
+    have : max (offset_pr f_h g_h + 1 + n + 1) (highest_var p_f) = offset_pr f_h g_h + 1 + n + 1 := by
       simp_arith
-      have : highest_var p_f ≤ offset f_h g_h := by simp [offset]
+      have : highest_var p_f ≤ offset_pr f_h g_h := by simp [offset_pr ]
       exact Nat.le_trans this (Nat.le_add_right _ (n + 2))
     rewrite [this]
-    have : (max (offset f_h g_h + 1 + (n + 1)) (offset f_h g_h + 1 + n + 1)) = offset f_h g_h + 1 + n + 1 := by
+    have : (max (offset_pr f_h g_h + 1 + (n + 1)) (offset_pr f_h g_h + 1 + n + 1)) = offset_pr f_h g_h + 1 + n + 1 := by
       repeat rewrite [←Nat.add_assoc]
       exact Nat.max_self _
     rewrite [this]
     simp_arith
 
-theorem prec_program_2_highest_var : highest_var (prec_program_2 f_h g_h) = offset f_h g_h + 1 + n := by
+theorem prec_program_2_highest_var : highest_var (prec_program_2 f_h g_h) = offset_pr f_h g_h + 1 + n := by
 
   simp [prec_program_2]
   cases n
   case zero =>
     simp [highest_var]
     constructor
-    simp [offset]
-    have : highest_var p_g ≤ offset f_h g_h := by simp [offset]
+    simp [offset_pr ]
+    have : highest_var p_g ≤ offset_pr f_h g_h := by simp [offset_pr ]
     exact Nat.le_trans this (Nat.le_add_right _ 1)
   case succ n =>
     simp [highest_var, highest_var_clear, highest_var_setup]
-    have : max (n + 3) (offset f_h g_h + 1 + n + 1) = offset f_h g_h + 1 + n + 1 := by simp_arith [offset]
+    have : max (n + 3) (offset_pr f_h g_h + 1 + n + 1) = offset_pr f_h g_h + 1 + n + 1 := by simp_arith [offset_pr ]
     rewrite [this]
-    have : max (offset f_h g_h + 1) (max 2 (highest_var p_g)) = offset f_h g_h + 1 := by
-      have h1 : offset f_h g_h + 1 ≥ 2 := by simp [offset]
-      have h2 : offset f_h g_h + 1 ≥ highest_var p_g := by exact calc
-        highest_var p_g ≤ offset f_h g_h := by simp [offset]
-                      _ ≤ offset f_h g_h + 1 := by simp_arith
+    have : max (offset_pr f_h g_h + 1) (max 2 (highest_var p_g)) = offset_pr f_h g_h + 1 := by
+      have h1 : offset_pr f_h g_h + 1 ≥ 2 := by simp [offset_pr ]
+      have h2 : offset_pr f_h g_h + 1 ≥ highest_var p_g := by exact calc
+        highest_var p_g ≤ offset_pr f_h g_h := by simp [offset_pr ]
+                      _ ≤ offset_pr f_h g_h + 1 := by simp_arith
       have := Nat.max_le_of_le_of_le h1 h2
       rewrite [Nat.max_comm]
       exact Nat.max_eq_right this
     rewrite [this]
-    have : max (offset f_h g_h + 1 + n + 1) (offset f_h g_h + 1) = offset f_h g_h + 1 + n + 1 := by
+    have : max (offset_pr f_h g_h + 1 + n + 1) (offset_pr f_h g_h + 1) = offset_pr f_h g_h + 1 + n + 1 := by
       simp
-      -- offset f_h g_h ≤ offset f_h g_h + 1 + n
+      -- offset_pr f_h g_h ≤ offset_pr f_h g_h + 1 + n
       exact calc
-        offset f_h g_h ≤ offset f_h g_h := by exact Nat.le_refl (offset f_h g_h)
-                     _ ≤ offset f_h g_h + (1 + n) := by simp
-                     _ = offset f_h g_h + 1 + n := by rw [Nat.add_assoc]
+        offset_pr f_h g_h ≤ offset_pr f_h g_h := by exact Nat.le_refl (offset_pr f_h g_h)
+                     _ ≤ offset_pr f_h g_h + (1 + n) := by simp
+                     _ = offset_pr f_h g_h + 1 + n := by rw [Nat.add_assoc]
     rw [this, Nat.add_assoc]
 
-theorem prec_program_3_highest_var : highest_var (prec_program_3 f_h g_h) = offset f_h g_h + 1 + n := by
+theorem prec_program_3_highest_var : highest_var (prec_program_3 f_h g_h) = offset_pr f_h g_h + 1 + n := by
   simp [prec_program_3]
   cases n
   case zero =>
@@ -199,24 +199,24 @@ theorem prec_program_3_highest_var : highest_var (prec_program_3 f_h g_h) = offs
   case succ n =>
     simp [highest_var]
     rewrite [highest_var_clear, highest_var_clear_Z, highest_var_setup]
-    simp_arith [offset]
+    simp_arith [offset_pr ]
 
-theorem prec_program_highest_var : highest_var (prec_program f_h g_h) = offset f_h g_h + 1 + n := by
+theorem prec_program_highest_var : highest_var (prec_program f_h g_h) = offset_pr f_h g_h + 1 + n := by
   simp [prec_program]
   repeat rewrite [highest_var_concat]
   rewrite [prec_program_1_highest_var, prec_program_2_highest_var, prec_program_3_highest_var]
   repeat rw [Nat.max_self]
 
 theorem execution_from_state_prec_program_1_1 (v : VectNat (n + 1)) :
-    execution_from_state (0 :: (v.toList ++ 0 :: (List.zeros (offset f_h g_h - (n + 2)) ++  0 :: List.zeros n))) (store_X_1_to_X_succ_n (offset f_h g_h + 1) n)
-      = 0 :: v.toList ++ 0 :: List.zeros (offset f_h g_h - (n + 2)) ++ v.toList := by
-  let c :=  offset f_h g_h - (n + 2)
-  have : offset f_h g_h - (n + 2) = c := rfl
+    execution_from_state (0 :: (v.toList ++ 0 :: (List.zeros (offset_pr f_h g_h - (n + 2)) ++  0 :: List.zeros n))) (store_X_1_to_X_succ_n (offset_pr f_h g_h + 1) n)
+      = 0 :: v.toList ++ 0 :: List.zeros (offset_pr f_h g_h - (n + 2)) ++ v.toList := by
+  let c :=  offset_pr f_h g_h - (n + 2)
+  have : offset_pr f_h g_h - (n + 2) = c := rfl
   rewrite [this]
-  have : offset f_h g_h + 1 = c + n + 3 := by
+  have : offset_pr f_h g_h + 1 = c + n + 3 := by
     simp [c]
     rewrite [Nat.add_assoc]
-    have : n + 2 ≤ offset f_h g_h := Nat.le_max_left _ _
+    have : n + 2 ≤ offset_pr f_h g_h := Nat.le_max_left _ _
     rw [Nat.sub_add_cancel this]
   rewrite [this]
   let w := 0 :: List.zeros c
@@ -230,13 +230,13 @@ theorem execution_from_state_prec_program_1_1 (v : VectNat (n + 1)) :
   exact this
 
 theorem execution_from_state_prec_program_1_2 (v : VectNat (n + 1)) :
-    execution_from_state (0 :: v.toList ++ 0 :: List.zeros (offset f_h g_h - (n + 2)) ++ v.toList) (clear_X_j_to_X_n_plus_j 1 n)
-      = 0 :: List.zeros (n + 1) ++ 0 :: List.zeros (offset f_h g_h - (n + 2)) ++ v.toList := by
+    execution_from_state (0 :: v.toList ++ 0 :: List.zeros (offset_pr f_h g_h - (n + 2)) ++ v.toList) (clear_X_j_to_X_n_plus_j 1 n)
+      = 0 :: List.zeros (n + 1) ++ 0 :: List.zeros (offset_pr f_h g_h - (n + 2)) ++ v.toList := by
   have : highest_var (clear_X_j_to_X_n_plus_j 1 n) ≤ n + 1 := by
     have : highest_var (clear_X_j_to_X_n_plus_j 1 n) = n + 1 := highest_var_clear
     rewrite [this]
     exact Nat.le_refl _
-  have := @execution_from_state_gt_highest_append (clear_X_j_to_X_n_plus_j 1 n) (0 :: List.zeros (offset f_h g_h - (n + 2)) ++ Mathlib.Vector.toList v)
+  have := @execution_from_state_gt_highest_append (clear_X_j_to_X_n_plus_j 1 n) (0 :: List.zeros (offset_pr f_h g_h - (n + 2)) ++ Vector.toList v)
     (n + 1) ⟨0 :: v.toList, by simp⟩ this
   simp at this
   simp
@@ -244,26 +244,26 @@ theorem execution_from_state_prec_program_1_2 (v : VectNat (n + 1)) :
   simp
 
 theorem execution_from_state_prec_program_1_3 (v : VectNat (n + 1)) :
-    execution_from_state (0 :: List.zeros (n + 1) ++ 0 :: List.zeros (offset f_h g_h - (n + 2)) ++ v.toList) (match n with | 0 => p_f | n + 1 => setup_X_j_to_X_n_plus_j (offset f_h g_h + 1) 1 n ++ p_f)
-      = f v.tail :: v.tail.toList ++ 0 :: 0 :: List.zeros (offset f_h g_h - (n + 2)) ++ v.toList := by
+    execution_from_state (0 :: List.zeros (n + 1) ++ 0 :: List.zeros (offset_pr f_h g_h - (n + 2)) ++ v.toList) (match n with | 0 => p_f | n + 1 => setup_X_j_to_X_n_plus_j (offset_pr f_h g_h + 1) 1 n ++ p_f)
+      = f v.tail :: v.tail.toList ++ 0 :: 0 :: List.zeros (offset_pr f_h g_h - (n + 2)) ++ v.toList := by
   cases n
   case zero =>
     simp
-    have : 0 :: 0 :: 0 :: (List.zeros (offset f_h g_h - 2) ++ [v.head]) = 0 :: (0 :: 0 :: List.zeros (offset f_h g_h - 2)) ++ [v.head] := by simp
+    have : 0 :: 0 :: 0 :: (List.zeros (offset_pr f_h g_h - 2) ++ [v.head]) = 0 :: (0 :: 0 :: List.zeros (offset_pr f_h g_h - 2)) ++ [v.head] := by simp
     rewrite [this]
-    have z_h : 0 :: 0 :: List.zeros (offset f_h g_h - 2) = List.zeros (offset f_h g_h) := by
+    have z_h : 0 :: 0 :: List.zeros (offset_pr f_h g_h - 2) = List.zeros (offset_pr f_h g_h) := by
       repeat rewrite [←zeros_succ]
-      have : offset f_h g_h - 2 + 2 = offset f_h g_h := by
-        have : offset f_h g_h ≥ 2 := by simp [offset]
+      have : offset_pr f_h g_h - 2 + 2 = offset_pr f_h g_h := by
+        have : offset_pr f_h g_h ≥ 2 := by simp [offset_pr ]
         rw [Nat.sub_add_cancel this]
       rw [this]
     rewrite [z_h]
-    have := @cleanly_computable_append_zeros_append_xs 0 p_f f (offset f_h g_h) f_h v.toList Mathlib.Vector.nil (by simp [offset])
+    have := @cleanly_computable_append_zeros_append_xs 0 p_f f (offset_pr f_h g_h) f_h v.toList Vector.nil (by simp [offset_pr ])
     simp [init_state] at this
     simp
     rewrite [this]
     simp
-    have : 0 :: 0 :: (List.zeros (offset f_h g_h - 2) ++ [v.head]) = List.zeros (offset f_h g_h) ++ [v.head] := by
+    have : 0 :: 0 :: (List.zeros (offset_pr f_h g_h - 2) ++ [v.head]) = List.zeros (offset_pr f_h g_h) ++ [v.head] := by
       repeat rewrite [←List.cons_append]
       rw [z_h]
     rw [this]
@@ -271,79 +271,79 @@ theorem execution_from_state_prec_program_1_3 (v : VectNat (n + 1)) :
     let ⟨x :: xs, xs_l⟩ := v
     simp at xs_l
     rewrite [List.zeros_concat]
-    simp [concat_is_seq_execution, execution_from_state, Mathlib.Vector.tail]
-    have list_zeros : 0 :: 0 :: List.zeros (offset f_h g_h - (n + 1 + 2)) = List.zeros (offset f_h g_h - (n + 1)) := by
+    simp [concat_is_seq_execution, execution_from_state, Vector.tail]
+    have list_zeros : 0 :: 0 :: List.zeros (offset_pr f_h g_h - (n + 1 + 2)) = List.zeros (offset_pr f_h g_h - (n + 1)) := by
       repeat rewrite [←zeros_succ]
-      suffices h : offset f_h g_h - (n + 1 + 2) + 1 + 1 = offset f_h g_h - (n + 1) from by rw [h]
+      suffices h : offset_pr f_h g_h - (n + 1 + 2) + 1 + 1 = offset_pr f_h g_h - (n + 1) from by rw [h]
       rewrite [Nat.add_assoc, Nat.sub_add_eq]
       have : 1 + 1 = 2 := rfl
       rewrite [this]
-      suffices h : offset f_h g_h - (n + 1) ≥ 2 from Nat.sub_add_cancel h
-      suffices h : offset f_h g_h ≥ 2 + (n + 1) from by
+      suffices h : offset_pr f_h g_h - (n + 1) ≥ 2 from Nat.sub_add_cancel h
+      suffices h : offset_pr f_h g_h ≥ 2 + (n + 1) from by
         have := Nat.sub_le_sub_right h (n + 1)
         rewrite [Nat.add_sub_cancel 2 (n + 1)] at this
         assumption
       rewrite [Nat.add_comm 2 (n + 1)]
       exact by calc
-        offset f_h g_h ≥ n + 1 + 2 := by dsimp [offset]; exact Nat.le_max_left _ _
+        offset_pr f_h g_h ≥ n + 1 + 2 := by dsimp [offset_pr ]; exact Nat.le_max_left _ _
                      _ = n + 3 := by rw [Nat.add_assoc]
-    have : List.zeros (n + 1) ++ 0 :: 0 :: (List.zeros (offset f_h g_h - (n + 1 + 2)) ++ x :: xs)
-      = List.zeros (n + 1) ++ List.zeros (offset f_h g_h - (n + 1)) ++ x :: xs := by exact calc
-            List.zeros (n + 1) ++ 0 :: 0 :: (List.zeros (offset f_h g_h - (n + 1 + 2)) ++x :: xs)
-                = List.zeros (n + 1) ++ (0 :: 0 :: List.zeros (offset f_h g_h - (n + 1 + 2))) ++ x :: xs := by simp
-              _ = List.zeros (n + 1) ++ List.zeros (offset f_h g_h - (n + 1)) ++ x :: xs := by rw [list_zeros]
+    have : List.zeros (n + 1) ++ 0 :: 0 :: (List.zeros (offset_pr f_h g_h - (n + 1 + 2)) ++ x :: xs)
+      = List.zeros (n + 1) ++ List.zeros (offset_pr f_h g_h - (n + 1)) ++ x :: xs := by exact calc
+            List.zeros (n + 1) ++ 0 :: 0 :: (List.zeros (offset_pr f_h g_h - (n + 1 + 2)) ++x :: xs)
+                = List.zeros (n + 1) ++ (0 :: 0 :: List.zeros (offset_pr f_h g_h - (n + 1 + 2))) ++ x :: xs := by simp
+              _ = List.zeros (n + 1) ++ List.zeros (offset_pr f_h g_h - (n + 1)) ++ x :: xs := by rw [list_zeros]
     rewrite [this]
-    have : (xs ++ 0 :: 0 :: (List.zeros (offset f_h g_h - (n + 1 + 2)) ++ x :: xs))
-      = xs ++ List.zeros (offset f_h g_h - (n + 1)) ++ x :: xs := by exact calc
-            xs ++ 0 :: 0 :: (List.zeros (offset f_h g_h - (n + 1 + 2)) ++ x :: xs)
-                = xs ++ (0 :: 0 :: List.zeros (offset f_h g_h - (n + 1 + 2))) ++ x :: xs := by simp
-              _ = xs ++ List.zeros (offset f_h g_h - (n + 1)) ++ x :: xs := by rw [list_zeros]
+    have : (xs ++ 0 :: 0 :: (List.zeros (offset_pr f_h g_h - (n + 1 + 2)) ++ x :: xs))
+      = xs ++ List.zeros (offset_pr f_h g_h - (n + 1)) ++ x :: xs := by exact calc
+            xs ++ 0 :: 0 :: (List.zeros (offset_pr f_h g_h - (n + 1 + 2)) ++ x :: xs)
+                = xs ++ (0 :: 0 :: List.zeros (offset_pr f_h g_h - (n + 1 + 2))) ++ x :: xs := by simp
+              _ = xs ++ List.zeros (offset_pr f_h g_h - (n + 1)) ++ x :: xs := by rw [list_zeros]
     rewrite [this]
     --
-    have : List.zeros (n + 1) ++ List.zeros (offset f_h g_h - (n + 1)) ++ x :: xs
-      = List.zeros (n + 1) ++ (List.zeros (offset f_h g_h - (n + 1)) ++ [x]) ++ xs := by rewrite [List.append_assoc] ; simp
+    have : List.zeros (n + 1) ++ List.zeros (offset_pr f_h g_h - (n + 1)) ++ x :: xs
+      = List.zeros (n + 1) ++ (List.zeros (offset_pr f_h g_h - (n + 1)) ++ [x]) ++ xs := by rewrite [List.append_assoc] ; simp
     rewrite [this]
-    have : (List.zeros (offset f_h g_h - (n + 1)) ++ [x]).length = offset f_h g_h - n := by
+    have : (List.zeros (offset_pr f_h g_h - (n + 1)) ++ [x]).length = offset_pr f_h g_h - n := by
       simp
       rewrite [Nat.sub_add_eq]
-      suffices h : offset f_h g_h - n ≥ 1 from Nat.sub_add_cancel h
+      suffices h : offset_pr f_h g_h - n ≥ 1 from Nat.sub_add_cancel h
       exact calc
-        offset f_h g_h - n ≥ (n + 1 + 2) - n := by
-          dsimp [offset]
+        offset_pr f_h g_h - n ≥ (n + 1 + 2) - n := by
+          dsimp [offset_pr ]
           exact Nat.sub_le_sub_right (Nat.le_max_left (n + 1 + 2) (max (highest_var p_f) (highest_var p_g))) n
         _ ≥ 1 := by
           rewrite [Nat.add_comm, Nat.add_comm n, ←Nat.add_assoc, Nat.add_sub_cancel]
           simp_arith
-    have := lemma_setup_X_1 (offset f_h g_h - n) n ⟨List.zeros (offset f_h g_h - (n + 1)) ++ [x], this⟩ ⟨xs, xs_l⟩
-    dsimp [Mathlib.Vector.toList] at this
+    have := lemma_setup_X_1 (offset_pr f_h g_h - n) n ⟨List.zeros (offset_pr f_h g_h - (n + 1)) ++ [x], this⟩ ⟨xs, xs_l⟩
+    dsimp [Vector.toList] at this
 
-    have lemm_eq : n + (offset f_h g_h - n) + 1 = offset f_h g_h + 1 := by
+    have lemm_eq : n + (offset_pr f_h g_h - n) + 1 = offset_pr f_h g_h + 1 := by
       simp_arith
       rewrite [Nat.add_comm]
-      suffices h : n ≤ offset f_h g_h from by exact Nat.sub_add_cancel h
+      suffices h : n ≤ offset_pr f_h g_h from by exact Nat.sub_add_cancel h
       exact by calc
         n ≤ n + 1 + 2 := by simp_arith
-        _  ≤ offset f_h g_h := by dsimp [offset]; exact Nat.le_max_left _ _
+        _  ≤ offset_pr f_h g_h := by dsimp [offset_pr ]; exact Nat.le_max_left _ _
     rewrite [lemm_eq] at this
     rewrite [this]
     rewrite [←List.cons_append, ←List.cons_append]
     rewrite [←List.append_assoc]
-    have : offset f_h g_h - (n + 1) ≥ highest_var p_f - (n + 1) := by
-      suffices h : offset f_h g_h ≥ highest_var p_f from Nat.sub_le_sub_right h (n + 1)
-      simp [offset]
+    have : offset_pr f_h g_h - (n + 1) ≥ highest_var p_f - (n + 1) := by
+      suffices h : offset_pr f_h g_h ≥ highest_var p_f from Nat.sub_le_sub_right h (n + 1)
+      simp [offset_pr ]
     have := cleanly_computable_append_zeros_append_xs f_h ([x] ++ xs) ⟨xs, xs_l⟩ this
     simp [init_state] at this
     simp
     rw [this]
 
 theorem execution_from_state_prec_program_1 (v : VectNat (n + 1)) :
-    execution_from_state (0 :: v.toList ++ 0 :: List.zeros (offset f_h g_h - (n + 2)) ++ 0 :: List.zeros n) (prec_program_1 f_h g_h)
-      = f v.tail :: v.tail.toList ++ 0 :: 0 :: List.zeros (offset f_h g_h - (n + 2)) ++ v.toList := by
-  let p_1_1 := store_X_1_to_X_succ_n (offset f_h g_h + 1) n
+    execution_from_state (0 :: v.toList ++ 0 :: List.zeros (offset_pr f_h g_h - (n + 2)) ++ 0 :: List.zeros n) (prec_program_1 f_h g_h)
+      = f v.tail :: v.tail.toList ++ 0 :: 0 :: List.zeros (offset_pr f_h g_h - (n + 2)) ++ v.toList := by
+  let p_1_1 := store_X_1_to_X_succ_n (offset_pr f_h g_h + 1) n
   let p_1_2 := clear_X_j_to_X_n_plus_j 1 n
   let p_1_3 := match n with
     | 0 => p_f
-    | n + 1 => setup_X_j_to_X_n_plus_j (offset f_h g_h + 1) 1 n ++ p_f
+    | n + 1 => setup_X_j_to_X_n_plus_j (offset_pr f_h g_h + 1) 1 n ++ p_f
   have : prec_program_1 f_h g_h = p_1_1 ++ p_1_2 ++ p_1_3:= by
     dsimp [prec_program_1, p_1_1, p_1_2, p_1_3]
 
@@ -356,26 +356,26 @@ theorem execution_from_state_prec_program_1 (v : VectNat (n + 1)) :
   simp
 
 theorem execution_from_state_prec_program_2_1 (R k : Nat) (v : VectNat (n + 1)) :
-    execution_from_state (R :: k :: 0 :: v.tail.toList ++ List.zeros (offset f_h g_h - (n + 2)) ++ v.toList) (X 2 += X 0)
-      = R :: k :: R :: v.tail.toList ++ List.zeros (offset f_h g_h - (n + 2)) ++ v.toList := by
+    execution_from_state (R :: k :: 0 :: v.tail.toList ++ List.zeros (offset_pr f_h g_h - (n + 2)) ++ v.toList) (X 2 += X 0)
+      = R :: k :: R :: v.tail.toList ++ List.zeros (offset_pr f_h g_h - (n + 2)) ++ v.toList := by
   exact calc
-      execution_from_state (R :: k :: 0 :: v.tail.toList ++ List.zeros (offset f_h g_h - (n + 2)) ++ v.toList) (X 2 += X 0)
-    = execution_from_state ([R, k] ++ 0 :: (v.tail.toList ++ List.zeros (offset f_h g_h - (n + 2)) ++ v.toList)) (X 2 += X 0) := by simp
-  _ = R :: k :: R :: v.tail.toList ++ List.zeros (offset f_h g_h - (n + 2)) ++ v.toList := by
+      execution_from_state (R :: k :: 0 :: v.tail.toList ++ List.zeros (offset_pr f_h g_h - (n + 2)) ++ v.toList) (X 2 += X 0)
+    = execution_from_state ([R, k] ++ 0 :: (v.tail.toList ++ List.zeros (offset_pr f_h g_h - (n + 2)) ++ v.toList)) (X 2 += X 0) := by simp
+  _ = R :: k :: R :: v.tail.toList ++ List.zeros (offset_pr f_h g_h - (n + 2)) ++ v.toList := by
       have : [R, k].length = 2 := rfl
       rewrite [inc_X_i_X_j_adds_value this]
       simp [value_at]
 
 theorem execution_from_state_prec_program_2_2 (R k : Nat) (v : VectNat (n + 1)) :
-    execution_from_state (R :: k :: R :: v.tail.toList ++ List.zeros (offset f_h g_h - (n + 2)) ++ v.toList) (CLEAR X 0)
-      = 0 :: k :: R :: v.tail.toList ++ List.zeros (offset f_h g_h - (n + 2)) ++ v.toList := by
+    execution_from_state (R :: k :: R :: v.tail.toList ++ List.zeros (offset_pr f_h g_h - (n + 2)) ++ v.toList) (CLEAR X 0)
+      = 0 :: k :: R :: v.tail.toList ++ List.zeros (offset_pr f_h g_h - (n + 2)) ++ v.toList := by
   simp [execution_from_state, clear_value]
 
 theorem execution_from_state_prec_program_2_3 (R k : Nat) (v : VectNat (n + 1)) :
-    execution_from_state (0 :: k :: R :: v.tail.toList ++ List.zeros (offset f_h g_h - (n + 2)) ++ v.toList) p_g
-      = g (k ::ᵥ R ::ᵥ v.tail) :: k :: R :: v.tail.toList ++ List.zeros (offset f_h g_h - (n + 2)) ++ v.toList := by
-  have : offset f_h g_h - (n + 2) ≥ highest_var p_g - (n + 2) := by
-    have : offset f_h g_h ≥ highest_var p_g := by simp [offset]
+    execution_from_state (0 :: k :: R :: v.tail.toList ++ List.zeros (offset_pr f_h g_h - (n + 2)) ++ v.toList) p_g
+      = g (k ::ᵥ R ::ᵥ v.tail) :: k :: R :: v.tail.toList ++ List.zeros (offset_pr f_h g_h - (n + 2)) ++ v.toList := by
+  have : offset_pr f_h g_h - (n + 2) ≥ highest_var p_g - (n + 2) := by
+    have : offset_pr f_h g_h ≥ highest_var p_g := by simp [offset_pr ]
     exact Nat.sub_le_sub_right this (n + 2)
   have := cleanly_computable_append_zeros_append_xs g_h v.toList (k ::ᵥ R ::ᵥ v.tail) this
   simp [init_state] at this
@@ -383,18 +383,18 @@ theorem execution_from_state_prec_program_2_3 (R k : Nat) (v : VectNat (n + 1)) 
   exact this
 
 theorem execution_from_state_prec_program_2_4 (R k : Nat) (v : VectNat (n + 1)) :
-    execution_from_state (g (k ::ᵥ R ::ᵥ v.tail) :: k :: R :: v.tail.toList ++ List.zeros (offset f_h g_h - (n + 2)) ++ v.toList) (CLEAR X 2)
-      = g (k ::ᵥ R ::ᵥ v.tail) :: k :: 0 :: v.tail.toList ++ List.zeros (offset f_h g_h - (n + 2)) ++ v.toList := by
+    execution_from_state (g (k ::ᵥ R ::ᵥ v.tail) :: k :: R :: v.tail.toList ++ List.zeros (offset_pr f_h g_h - (n + 2)) ++ v.toList) (CLEAR X 2)
+      = g (k ::ᵥ R ::ᵥ v.tail) :: k :: 0 :: v.tail.toList ++ List.zeros (offset_pr f_h g_h - (n + 2)) ++ v.toList := by
   simp [execution_from_state, clear_value]
 
 theorem execution_from_state_prec_program_2_5 (R k : Nat) (v : VectNat (n + 1)) :
-    execution_from_state (g (k ::ᵥ R ::ᵥ v.tail) :: k :: 0 :: v.tail.toList ++ List.zeros (offset f_h g_h - (n + 2)) ++ v.toList) (INC X 1)
-      = g (k ::ᵥ R ::ᵥ v.tail) :: (k + 1) :: 0 :: v.tail.toList ++ List.zeros (offset f_h g_h - (n + 2)) ++ v.toList := by
+    execution_from_state (g (k ::ᵥ R ::ᵥ v.tail) :: k :: 0 :: v.tail.toList ++ List.zeros (offset_pr f_h g_h - (n + 2)) ++ v.toList) (INC X 1)
+      = g (k ::ᵥ R ::ᵥ v.tail) :: (k + 1) :: 0 :: v.tail.toList ++ List.zeros (offset_pr f_h g_h - (n + 2)) ++ v.toList := by
   simp [execution_from_state, inc_value]
 
 theorem execution_from_state_prec_program_loop_inner (R k : Nat) (v : VectNat (n + 1)) :
-  execution_from_state (R :: k :: 0 :: v.tail.toList ++ List.zeros (offset f_h g_h - (n + 2)) ++ v.toList) (X 2 += X 0 ++ CLEAR X 0 ++ p_g ++ CLEAR X 2 ++ INC X 1)
-      = g (k ::ᵥ R ::ᵥ v.tail) :: (k + 1) :: 0 :: v.tail.toList ++ List.zeros (offset f_h g_h - (n + 2)) ++ v.toList := by
+  execution_from_state (R :: k :: 0 :: v.tail.toList ++ List.zeros (offset_pr f_h g_h - (n + 2)) ++ v.toList) (X 2 += X 0 ++ CLEAR X 0 ++ p_g ++ CLEAR X 2 ++ INC X 1)
+      = g (k ::ᵥ R ::ᵥ v.tail) :: (k + 1) :: 0 :: v.tail.toList ++ List.zeros (offset_pr f_h g_h - (n + 2)) ++ v.toList := by
   repeat rewrite [concat_is_seq_execution]
   repeat rewrite [seq_execution_unfold]
   rw [execution_from_state_prec_program_2_1, execution_from_state_prec_program_2_2,
@@ -402,31 +402,31 @@ theorem execution_from_state_prec_program_loop_inner (R k : Nat) (v : VectNat (n
       execution_from_state_prec_program_2_5]
 
 theorem execution_from_state_prec_program_loop (v : VectNat (n + 1)) :
-  execution_from_state (f v.tail :: 0 :: 0 :: v.tail.toList ++ List.zeros (offset f_h g_h - (n + 2)) ++ v.toList)
-      (LOOP X (offset f_h g_h + 1) DO (X 2 += X 0 ++ CLEAR X 0 ++ p_g ++ CLEAR X 2 ++ INC X 1) END)
-    = (v.head.rec (f v.tail) fun y IH => g (y ::ᵥ IH ::ᵥ v.tail)) :: v.head :: 0 :: v.tail.toList ++ List.zeros (offset f_h g_h - (n + 2)) ++ v.toList := by
+  execution_from_state (f v.tail :: 0 :: 0 :: v.tail.toList ++ List.zeros (offset_pr f_h g_h - (n + 2)) ++ v.toList)
+      (LOOP X (offset_pr f_h g_h + 1) DO (X 2 += X 0 ++ CLEAR X 0 ++ p_g ++ CLEAR X 2 ++ INC X 1) END)
+    = (v.head.rec (f v.tail) fun y IH => g (y ::ᵥ IH ::ᵥ v.tail)) :: v.head :: 0 :: v.tail.toList ++ List.zeros (offset_pr f_h g_h - (n + 2)) ++ v.toList := by
   let ⟨x :: xs, xs_l⟩ := v
 
   simp at xs_l
-  dsimp [Mathlib.Vector.tail, Mathlib.Vector.head]
+  dsimp [Vector.tail, Vector.head]
   simp [execution_from_state]
-  have : value_at (f ⟨xs, xs_l⟩ :: 0 :: 0 :: (xs ++ (List.zeros (offset f_h g_h - (n + 2)) ++ x :: xs))) (offset f_h g_h + 1)
+  have : value_at (f ⟨xs, xs_l⟩ :: 0 :: 0 :: (xs ++ (List.zeros (offset_pr f_h g_h - (n + 2)) ++ x :: xs))) (offset_pr f_h g_h + 1)
       = x := by
     exact calc
-          value_at (f ⟨xs, xs_l⟩ :: 0 :: 0 :: (xs ++ (List.zeros (offset f_h g_h - (n + 2)) ++ x :: xs))) (offset f_h g_h + 1)
-        = value_at ((f ⟨xs, xs_l⟩ :: 0 :: 0 :: xs ++ List.zeros (offset f_h g_h - (n + 2))) ++ x :: xs) (offset f_h g_h + 1) := by simp
+          value_at (f ⟨xs, xs_l⟩ :: 0 :: 0 :: (xs ++ (List.zeros (offset_pr f_h g_h - (n + 2)) ++ x :: xs))) (offset_pr f_h g_h + 1)
+        = value_at ((f ⟨xs, xs_l⟩ :: 0 :: 0 :: xs ++ List.zeros (offset_pr f_h g_h - (n + 2))) ++ x :: xs) (offset_pr f_h g_h + 1) := by simp
       _ = x := by
-          have : (f ⟨xs, xs_l⟩ :: 0 :: 0 :: xs ++ List.zeros (offset f_h g_h - (n + 2))).length = offset f_h g_h + 1 := by
+          have : (f ⟨xs, xs_l⟩ :: 0 :: 0 :: xs ++ List.zeros (offset_pr f_h g_h - (n + 2))).length = offset_pr f_h g_h + 1 := by
             simp [xs_l]
             rewrite [Nat.add_assoc, Nat.add_comm _ 2, ←Nat.add_assoc, Nat.add_comm, Nat.add_comm 2 n]
-            suffices h : offset f_h g_h ≥ n + 2 from Nat.sub_add_cancel h
-            simp [offset]
+            suffices h : offset_pr f_h g_h ≥ n + 2 from Nat.sub_add_cancel h
+            simp [offset_pr ]
           exact value_at_n this
 
   rewrite [this]
-  suffices h : ∀ k : Nat, loop_n_times k (f ⟨xs, xs_l⟩ :: 0 :: 0 :: (xs ++ (List.zeros (offset f_h g_h - (n + 2)) ++ x :: xs)))
+  suffices h : ∀ k : Nat, loop_n_times k (f ⟨xs, xs_l⟩ :: 0 :: 0 :: (xs ++ (List.zeros (offset_pr f_h g_h - (n + 2)) ++ x :: xs)))
       (X 2 += X 0 ++ CLEAR X 0 ++ p_g ++ CLEAR X 2 ++ INC X 1)
-      = Nat.rec (f ⟨xs, xs_l⟩) (fun y IH ↦ g (y ::ᵥ IH ::ᵥ ⟨xs, xs_l⟩)) k :: k :: 0 :: (xs ++ (List.zeros (offset f_h g_h - (n + 2)) ++ x :: xs)) from h x
+      = Nat.rec (f ⟨xs, xs_l⟩) (fun y IH ↦ g (y ::ᵥ IH ::ᵥ ⟨xs, xs_l⟩)) k :: k :: 0 :: (xs ++ (List.zeros (offset_pr f_h g_h - (n + 2)) ++ x :: xs)) from h x
   intro k
   induction k
   case zero =>
@@ -436,13 +436,13 @@ theorem execution_from_state_prec_program_loop (v : VectNat (n + 1)) :
     have := execution_from_state_prec_program_loop_inner f_h g_h
       (Nat.rec (f ⟨xs, xs_l⟩) (fun y IH ↦ g (y ::ᵥ IH ::ᵥ ⟨xs, xs_l⟩)) k)
       k ⟨x :: xs, by simp [xs_l]⟩
-    simp [Mathlib.Vector.tail, Mathlib.Vector.toList] at this
+    simp [Vector.tail, Vector.toList] at this
     simp
     rw [this]
 
 theorem execution_from_state_prec_program_2 (v : VectNat (n + 1)) :
-    execution_from_state (f v.tail :: v.tail.toList ++ 0 :: 0 :: List.zeros (offset f_h g_h - (n + 2)) ++ v.toList) (prec_program_2 f_h g_h)
-      = (v.head.rec (f v.tail) fun y IH => g (y ::ᵥ IH ::ᵥ v.tail)) :: v.head :: 0 :: v.tail.toList ++ List.zeros (offset f_h g_h - (n + 2)) ++ v.toList := by
+    execution_from_state (f v.tail :: v.tail.toList ++ 0 :: 0 :: List.zeros (offset_pr f_h g_h - (n + 2)) ++ v.toList) (prec_program_2 f_h g_h)
+      = (v.head.rec (f v.tail) fun y IH => g (y ::ᵥ IH ::ᵥ v.tail)) :: v.head :: 0 :: v.tail.toList ++ List.zeros (offset_pr f_h g_h - (n + 2)) ++ v.toList := by
   dsimp [prec_program_2]
   cases n
   case zero =>
@@ -456,12 +456,12 @@ theorem execution_from_state_prec_program_2 (v : VectNat (n + 1)) :
     repeat rewrite [seq_execution_unfold]
     suffices h : execution_from_state
       (execution_from_state
-        (f (Mathlib.Vector.tail v) ::
-          ((Mathlib.Vector.tail v).toList ++ 0 :: 0 :: List.zeros (offset f_h g_h - (n + 1 + 2)) ++
-            Mathlib.Vector.toList v))
+        (f (Vector.tail v) ::
+          ((Vector.tail v).toList ++ 0 :: 0 :: List.zeros (offset_pr f_h g_h - (n + 1 + 2)) ++
+            Vector.toList v))
         (clear_X_j_to_X_n_plus_j 1 n))
-          (setup_X_j_to_X_n_plus_j (offset f_h g_h + 1) 3 n)
-        = f v.tail :: 0 :: 0 :: v.tail.toList ++ List.zeros (offset f_h g_h - (n + 1 + 2)) ++ v.toList from by
+          (setup_X_j_to_X_n_plus_j (offset_pr f_h g_h + 1) 3 n)
+        = f v.tail :: 0 :: 0 :: v.tail.toList ++ List.zeros (offset_pr f_h g_h - (n + 1 + 2)) ++ v.toList from by
       rewrite [h]
       have := execution_from_state_prec_program_loop f_h g_h v
       simp [concat_is_seq_execution] at this
@@ -469,49 +469,49 @@ theorem execution_from_state_prec_program_2 (v : VectNat (n + 1)) :
       rw [this]
     let ⟨x :: xs, xs_l⟩ := v
     simp_arith at xs_l
-    dsimp [Mathlib.Vector.tail]
+    dsimp [Vector.tail]
 
     have := calc
-        execution_from_state (f ⟨xs, xs_l⟩ :: (xs ++ 0 :: 0 :: List.zeros (offset f_h g_h - (n + 1 + 2)) ++ x :: xs))
+        execution_from_state (f ⟨xs, xs_l⟩ :: (xs ++ 0 :: 0 :: List.zeros (offset_pr f_h g_h - (n + 1 + 2)) ++ x :: xs))
           (clear_X_j_to_X_n_plus_j 1 n)
-        = execution_from_state ((f ⟨xs, xs_l⟩ :: xs) ++ (0 :: 0 :: List.zeros (offset f_h g_h - (n + 1 + 2)) ++ x :: xs))
+        = execution_from_state ((f ⟨xs, xs_l⟩ :: xs) ++ (0 :: 0 :: List.zeros (offset_pr f_h g_h - (n + 1 + 2)) ++ x :: xs))
          (clear_X_j_to_X_n_plus_j 1 n) := by simp
       _ = (execution_from_state (f ⟨xs, xs_l⟩ :: xs) (clear_X_j_to_X_n_plus_j 1 n))
-        ++ 0 :: 0 :: List.zeros (offset f_h g_h - (n + 1 + 2)) ++ x :: xs := by
+        ++ 0 :: 0 :: List.zeros (offset_pr f_h g_h - (n + 1 + 2)) ++ x :: xs := by
           have h := @execution_from_state_gt_highest_append (clear_X_j_to_X_n_plus_j 1 n)
-            (0 :: 0 :: List.zeros (offset f_h g_h - (n + 1 + 2)) ++ x :: xs)
+            (0 :: 0 :: List.zeros (offset_pr f_h g_h - (n + 1 + 2)) ++ x :: xs)
             (n + 1) (f ⟨xs, xs_l⟩ ::ᵥ ⟨xs, xs_l⟩) (by rw [highest_var_clear])
           have : (f ⟨xs, xs_l⟩ ::ᵥ ⟨xs, xs_l⟩).toList = f ⟨xs, xs_l⟩ :: xs := by simp
           rewrite [this] at h
           rw [h]
           simp
-      _ = f ⟨xs, xs_l⟩ :: List.zeros (n + 1) ++ 0 :: 0 :: List.zeros (offset f_h g_h - (n + 1 + 2)) ++ x :: xs := by
+      _ = f ⟨xs, xs_l⟩ :: List.zeros (n + 1) ++ 0 :: 0 :: List.zeros (offset_pr f_h g_h - (n + 1 + 2)) ++ x :: xs := by
           suffices h : execution_from_state (f ⟨xs, xs_l⟩ :: xs) (clear_X_j_to_X_n_plus_j 1 n) = f ⟨xs, xs_l⟩ :: List.zeros (n + 1) from by rw [h]
           rw [clear_X_succ]
           let v' : VectNat (n + 1) := ⟨xs, xs_l⟩
           have : execution_from_state xs (clear_X_j_to_X_n_plus_j 0 n)
             = execution_from_state (v'.toList) (clear_X_j_to_X_n_plus_j 0 n) := by simp [v']
           rw [this, clear_X_lemma]
-      _ = f ⟨xs, xs_l⟩ ::(List.zeros (n + 1) ++ [0] ++ [0]) ++ List.zeros (offset f_h g_h - (n + 1 + 2)) ++ x :: xs := by simp
-      _ = f ⟨xs, xs_l⟩ :: List.zeros (n + 3) ++ List.zeros (offset f_h g_h - (n + 1 + 2)) ++ x :: xs := by rw [←List.zeros_concat, ←List.zeros_concat]
-      _ = f ⟨xs, xs_l⟩ ::  0 :: 0 :: List.zeros (n + 1) ++ List.zeros (offset f_h g_h - (n + 1 + 2)) ++ x :: xs := by rw [zeros_succ, zeros_succ]
-      _ = f ⟨xs, xs_l⟩ ::  (0 :: (0 :: (List.zeros (n + 1) ++ List.zeros (offset f_h g_h - (n + 1 + 2)) ++ [x] ++ xs))) := by simp
-      _ = f ⟨xs, xs_l⟩ ::  (0 :: (0 :: (List.zeros (n + 1) ++ (List.zeros (offset f_h g_h - (n + 1 + 2)) ++ [x]) ++ xs))) := by repeat rw [List.append_assoc]
+      _ = f ⟨xs, xs_l⟩ ::(List.zeros (n + 1) ++ [0] ++ [0]) ++ List.zeros (offset_pr f_h g_h - (n + 1 + 2)) ++ x :: xs := by simp
+      _ = f ⟨xs, xs_l⟩ :: List.zeros (n + 3) ++ List.zeros (offset_pr f_h g_h - (n + 1 + 2)) ++ x :: xs := by rw [←List.zeros_concat, ←List.zeros_concat]
+      _ = f ⟨xs, xs_l⟩ ::  0 :: 0 :: List.zeros (n + 1) ++ List.zeros (offset_pr f_h g_h - (n + 1 + 2)) ++ x :: xs := by rw [zeros_succ, zeros_succ]
+      _ = f ⟨xs, xs_l⟩ ::  (0 :: (0 :: (List.zeros (n + 1) ++ List.zeros (offset_pr f_h g_h - (n + 1 + 2)) ++ [x] ++ xs))) := by simp
+      _ = f ⟨xs, xs_l⟩ ::  (0 :: (0 :: (List.zeros (n + 1) ++ (List.zeros (offset_pr f_h g_h - (n + 1 + 2)) ++ [x]) ++ xs))) := by repeat rw [List.append_assoc]
 
     rewrite [this]
-    have : offset f_h g_h + 1 = (offset f_h g_h - 2) + 3 := by
-      suffices h : offset f_h g_h ≥ 2 from by exact calc
-        offset f_h g_h + 1 = (offset f_h g_h - 2 + 2) + 1 := by rw [Nat.sub_add_cancel h]
-                         _ = (offset f_h g_h - 2) + 3 := by simp_arith
-      simp_arith [offset]
+    have : offset_pr f_h g_h + 1 = (offset_pr f_h g_h - 2) + 3 := by
+      suffices h : offset_pr f_h g_h ≥ 2 from by exact calc
+        offset_pr f_h g_h + 1 = (offset_pr f_h g_h - 2 + 2) + 1 := by rw [Nat.sub_add_cancel h]
+                         _ = (offset_pr f_h g_h - 2) + 3 := by simp_arith
+      simp_arith [offset_pr ]
     rewrite [this]
     repeat rewrite [setup_X_succ]
-    have := lemma_setup (offset f_h g_h - (n + 1 + 2) + 1) n ⟨List.zeros (offset f_h g_h - (n + 1 + 2)) ++ [x], by simp⟩ ⟨xs, xs_l⟩
+    have := lemma_setup (offset_pr f_h g_h - (n + 1 + 2) + 1) n ⟨List.zeros (offset_pr f_h g_h - (n + 1 + 2)) ++ [x], by simp⟩ ⟨xs, xs_l⟩
     dsimp at this
-    have h_eq : n + (offset f_h g_h - (n + 1 + 2) + 1) = offset f_h g_h - 2 := by
+    have h_eq : n + (offset_pr f_h g_h - (n + 1 + 2) + 1) = offset_pr f_h g_h - 2 := by
       rewrite [Nat.add_comm (n + 1), Nat.add_comm, Nat.add_assoc, Nat.add_comm 1 n, Nat.sub_add_eq]
-      suffices h : offset f_h g_h - 2 ≥ n + 1 from Nat.sub_add_cancel h
-      have : offset f_h g_h ≥ n + 2 + 1 := by simp [offset]
+      suffices h : offset_pr f_h g_h - 2 ≥ n + 1 from Nat.sub_add_cancel h
+      have : offset_pr f_h g_h ≥ n + 2 + 1 := by simp [offset_pr ]
       have := Nat.sub_le_sub_right this 2
       have h : n + 2 + 1 - 2 = n + 1 := by simp
       rewrite [h] at this
@@ -521,8 +521,8 @@ theorem execution_from_state_prec_program_2 (v : VectNat (n + 1)) :
     simp
 
 theorem execution_from_state_prec_program_3_1 (R : Nat) (v : VectNat (n + 1)) :
-    execution_from_state (R :: v.head :: 0 :: v.tail.toList ++ List.zeros (offset f_h g_h - (n + 2)) ++ v.toList) (match (generalizing := false) n with | 0 => CLEAR X 1 | n + 1 => CLEAR X 1 ++ clear_X_j_to_X_n_plus_j 3 n)
-        = R :: 0 :: 0 :: List.zeros n ++ List.zeros (offset f_h g_h - (n + 2)) ++ v.toList := by
+    execution_from_state (R :: v.head :: 0 :: v.tail.toList ++ List.zeros (offset_pr f_h g_h - (n + 2)) ++ v.toList) (match (generalizing := false) n with | 0 => CLEAR X 1 | n + 1 => CLEAR X 1 ++ clear_X_j_to_X_n_plus_j 3 n)
+        = R :: 0 :: 0 :: List.zeros n ++ List.zeros (offset_pr f_h g_h - (n + 2)) ++ v.toList := by
   cases n
   case zero =>
     simp [execution_from_state, clear_value]
@@ -535,14 +535,14 @@ theorem execution_from_state_prec_program_3_1 (R : Nat) (v : VectNat (n + 1)) :
     rewrite [execution_from_state_gt_highest_append v.tail this]
     rewrite [clear_X_lemma]
     rewrite [←List.append_assoc]
-    rw [append_zeros_addition (n + 1) ((offset f_h g_h - (n + 1 + 2))) ((n + 1 + (offset f_h g_h - (n + 1 + 2)))) (by simp)]
+    rw [append_zeros_addition (n + 1) ((offset_pr f_h g_h - (n + 1 + 2))) ((n + 1 + (offset_pr f_h g_h - (n + 1 + 2)))) (by simp)]
 
 theorem execution_from_state_prec_program_3_2 (R : Nat) (v : VectNat (n + 1)) :
-    execution_from_state (R :: 0 :: 0 :: List.zeros n ++ List.zeros (offset f_h g_h - (n + 2)) ++ v.toList) (setup_X_j_to_X_n_plus_j (offset f_h g_h) 1 n)
-        = R :: v.toList ++ List.zeros (offset f_h g_h - (n + 1)) ++ v.toList := by
-  have h_eq : offset f_h g_h = offset f_h g_h - 1 + 1 := by
-    suffices h : offset f_h g_h ≥ 1 from (Nat.sub_add_cancel h).symm
-    simp_arith [offset]
+    execution_from_state (R :: 0 :: 0 :: List.zeros n ++ List.zeros (offset_pr f_h g_h - (n + 2)) ++ v.toList) (setup_X_j_to_X_n_plus_j (offset_pr f_h g_h) 1 n)
+        = R :: v.toList ++ List.zeros (offset_pr f_h g_h - (n + 1)) ++ v.toList := by
+  have h_eq : offset_pr f_h g_h = offset_pr f_h g_h - 1 + 1 := by
+    suffices h : offset_pr f_h g_h ≥ 1 from (Nat.sub_add_cancel h).symm
+    simp_arith [offset_pr ]
   rewrite [h_eq]
   repeat rewrite [List.cons_append]
   rewrite [setup_X_succ]
@@ -550,23 +550,23 @@ theorem execution_from_state_prec_program_3_2 (R : Nat) (v : VectNat (n + 1)) :
   rewrite [←zeros_succ, ←zeros_succ, List.zeros_concat, h_eq.symm]
   simp
   rewrite [←List.cons_append, ←zeros_succ]
-  have : offset f_h g_h - (n + 2) + 1 = offset f_h g_h - (n + 1) := by
+  have : offset_pr f_h g_h - (n + 2) + 1 = offset_pr f_h g_h - (n + 1) := by
     have : n + 2 = (n + 1) + 1 := rfl
     rewrite [this, Nat.sub_add_eq]
-    suffices h : offset f_h g_h - (n + 1) ≥ 1 from Nat.sub_add_cancel h
-    have : offset f_h g_h ≥ n + 2 := by simp [offset]
+    suffices h : offset_pr f_h g_h - (n + 1) ≥ 1 from Nat.sub_add_cancel h
+    have : offset_pr f_h g_h ≥ n + 2 := by simp [offset_pr ]
     have := Nat.sub_le_sub_right this (n + 1)
     have h : n + 2 - (n + 1) = 1 := by simp_arith
     rewrite [h] at this
     assumption
   rewrite [this]
-  have : (List.zeros (offset f_h g_h - (n + 1))).length = offset f_h g_h - (n + 1) := by simp
-  have h_l := lemma_setup (offset f_h g_h - (n + 1)) n ⟨List.zeros (offset f_h g_h - (n + 1)), this⟩ v
-  have : n + (offset f_h g_h - (n + 1)) = offset f_h g_h - 1 := by
+  have : (List.zeros (offset_pr f_h g_h - (n + 1))).length = offset_pr f_h g_h - (n + 1) := by simp
+  have h_l := lemma_setup (offset_pr f_h g_h - (n + 1)) n ⟨List.zeros (offset_pr f_h g_h - (n + 1)), this⟩ v
+  have : n + (offset_pr f_h g_h - (n + 1)) = offset_pr f_h g_h - 1 := by
     rewrite [Nat.add_comm n 1]
     rewrite [Nat.add_comm, Nat.sub_add_eq]
-    suffices h : offset f_h g_h - 1 ≥ n from Nat.sub_add_cancel h
-    have : offset f_h g_h ≥ n + 1 := by simp [offset]
+    suffices h : offset_pr f_h g_h - 1 ≥ n from Nat.sub_add_cancel h
+    have : offset_pr f_h g_h ≥ n + 1 := by simp [offset_pr ]
     have := Nat.sub_le_sub_right this 1
     rewrite [Nat.add_sub_cancel] at this
     assumption
@@ -576,15 +576,15 @@ theorem execution_from_state_prec_program_3_2 (R : Nat) (v : VectNat (n + 1)) :
   rw [h_l]
 
 theorem execution_from_state_prec_program_3_3 (R : Nat) (v : VectNat (n + 1)) :
-    execution_from_state (R :: v.toList ++ List.zeros (offset f_h g_h - (n + 1)) ++ v.toList) (clear_Z_0_to_Z_n (offset f_h g_h + 1) n)
-        = R :: v.toList ++ List.zeros (offset f_h g_h) := by
-  have : (R :: v.toList ++ List.zeros (offset f_h g_h - (n + 1))).length = offset f_h g_h + 1 := by simp [offset]
+    execution_from_state (R :: v.toList ++ List.zeros (offset_pr f_h g_h - (n + 1)) ++ v.toList) (clear_Z_0_to_Z_n (offset_pr f_h g_h + 1) n)
+        = R :: v.toList ++ List.zeros (offset_pr f_h g_h) := by
+  have : (R :: v.toList ++ List.zeros (offset_pr f_h g_h - (n + 1))).length = offset_pr f_h g_h + 1 := by simp [offset_pr ]
   rewrite [clear_Z_lemma v this]
-  simp [offset]
+  simp [offset_pr ]
 
 theorem execution_from_state_prec_program_3 (v : VectNat (n + 1)) :
-  execution_from_state ((v.head.rec (f v.tail) fun y IH => g (y ::ᵥ IH ::ᵥ v.tail)) :: v.head :: 0 :: v.tail.toList ++ List.zeros (offset f_h g_h - (n + 2)) ++ v.toList) (prec_program_3 f_h g_h)
-    = (v.head.rec (f v.tail) fun y IH => g (y ::ᵥ IH ::ᵥ v.tail)) :: v.toList ++ List.zeros (offset f_h g_h) := by
+  execution_from_state ((v.head.rec (f v.tail) fun y IH => g (y ::ᵥ IH ::ᵥ v.tail)) :: v.head :: 0 :: v.tail.toList ++ List.zeros (offset_pr f_h g_h - (n + 2)) ++ v.toList) (prec_program_3 f_h g_h)
+    = (v.head.rec (f v.tail) fun y IH => g (y ::ᵥ IH ::ᵥ v.tail)) :: v.toList ++ List.zeros (offset_pr f_h g_h) := by
   dsimp [prec_program_3]
   repeat rewrite [concat_is_seq_execution]
   simp [execution_from_state]
@@ -594,8 +594,8 @@ theorem execution_from_state_prec_program_3 (v : VectNat (n + 1)) :
     execution_from_state_prec_program_3_3]
 
 theorem execution_from_state_prec_program (v : VectNat (n + 1)) :
-    execution_from_state (0 :: v.toList ++ 0 :: List.zeros (offset f_h g_h - (n + 2)) ++ 0 :: List.zeros n) (prec_program f_h g_h)
-      = (v.head.rec (f v.tail) fun y IH => g (y ::ᵥ IH ::ᵥ v.tail)) :: v.toList ++ List.zeros (offset f_h g_h) := by
+    execution_from_state (0 :: v.toList ++ 0 :: List.zeros (offset_pr f_h g_h - (n + 2)) ++ 0 :: List.zeros n) (prec_program f_h g_h)
+      = (v.head.rec (f v.tail) fun y IH => g (y ::ᵥ IH ::ᵥ v.tail)) :: v.toList ++ List.zeros (offset_pr f_h g_h) := by
   dsimp [prec_program]
   repeat rewrite [concat_is_seq_execution]
   simp [execution_from_state]
@@ -612,26 +612,207 @@ theorem prec_is_loop_computable_cleanly : loop_computable_cleanly f
   exists prec_program f_h g_h
   intro v
   rewrite [prec_program_highest_var]
-  have : offset f_h g_h + 1 + n - (n + 1) = offset f_h g_h := by
+  have : offset_pr f_h g_h + 1 + n - (n + 1) = offset_pr f_h g_h := by
     rewrite [Nat.add_assoc, Nat.add_comm 1 n]
     rw [Nat.add_sub_cancel]
   rewrite [this]
-  have : offset f_h g_h = offset f_h g_h - (n + 2) + (n + 1) + 1 := by
+  have : offset_pr f_h g_h = offset_pr f_h g_h - (n + 2) + (n + 1) + 1 := by
     rewrite [Nat.add_assoc]
-    suffices h : offset f_h g_h ≥ n + 2 from (Nat.sub_add_cancel h).symm
-    simp [offset]
-  have : init_state v ++ List.zeros (offset f_h g_h)
-      = 0 :: v.toList ++ 0 :: List.zeros (offset f_h g_h - (n + 2)) ++ 0 :: List.zeros n := by
+    suffices h : offset_pr f_h g_h ≥ n + 2 from (Nat.sub_add_cancel h).symm
+    simp [offset_pr ]
+  have : init_state v ++ List.zeros (offset_pr f_h g_h)
+      = 0 :: v.toList ++ 0 :: List.zeros (offset_pr f_h g_h - (n + 2)) ++ 0 :: List.zeros n := by
     dsimp [init_state]
     rewrite [this]
     rewrite [zeros_succ]
-    rewrite [←append_zeros_addition (offset f_h g_h - (n + 2)) (n + 1) (offset f_h g_h - (n + 2) + (n + 1)) rfl]
+    rewrite [←append_zeros_addition (offset_pr f_h g_h - (n + 2)) (n + 1) (offset_pr f_h g_h - (n + 2) + (n + 1)) rfl]
     rewrite [zeros_succ]
     simp
   rewrite [this]
   rw [execution_from_state_prec_program]
 
 end prec_is_loop_computable_cleanly_proof
+
+section comp_is_loop_computable_cleanly_proof
+
+-- We introduce a section as to delimit the proof, but there won't be any
+-- variable declaration, to make everything more explicit.
+
+-- variable
+--   {n m: Nat}
+--   {f : VectNat n → Nat}
+--   (g : Fin n → VectNat m → Nat)
+--   (f_h : cleanly_computes p_f f)
+--   (p_g : Fin n → Program)
+--   (g_h : ∀ i, cleanly_computes (p_g i) (g i))
+
+def highest_var_p_g {n : Nat} (p_g : Fin n → Program) : Nat := match n with
+  | 0 => 0
+  | n + 1 =>
+    let p_g_succ_n := p_g ⟨n, Nat.lt_succ_self n⟩
+    let p_g' : Fin n → Program
+      | ⟨k, p⟩ => p_g ⟨k, Nat.lt_trans p (Nat.lt_succ_self n)⟩
+    max (highest_var p_g_succ_n) (highest_var_p_g p_g')
+
+-- -- A bit different from offset_prec. It needs to know m, n, p_g and p_f. It
+-- -- takes three explicit arguments: m, p_f and p_g (from which n is obtained).
+def offset_comp (m : Nat) (p_g : Fin n → Program) (p_f : Program) : Nat
+  := max (max n m) (max (highest_var p_f) (highest_var_p_g p_g))
+
+theorem highest_var_p_g_ge_highest_var_p_g_i {p_g : Fin n → Program} :
+    ∀ i : Fin n, highest_var (p_g i) ≤ highest_var_p_g p_g := by
+  induction n
+  case zero =>
+    intro ⟨_, _⟩
+    contradiction
+  case succ n n_ih =>
+    intro ⟨k, p⟩
+    let p_g' : Fin n → Program
+      | ⟨k, p⟩ => p_g ⟨k, Nat.lt_trans p (Nat.lt_succ_self n)⟩
+    have : highest_var_p_g p_g = max (highest_var (p_g ⟨n, Nat.lt_succ_self n⟩)) (highest_var_p_g p_g') := by dsimp [highest_var_p_g]
+    rewrite [this]
+    cases (Nat.decEq k n)
+    case isTrue h =>
+      have : (⟨k, p⟩ : Fin (n + 1)) = ⟨n, Nat.lt_succ_self n⟩ := Fin.eq_of_val_eq h
+      rewrite [this]
+      exact Nat.le_max_left _ _
+    case isFalse h =>
+      suffices h' : highest_var (p_g ⟨k, p⟩) ≤ highest_var_p_g p_g' from by simp [h']
+      have p' : k < n := by
+        cases (Nat.decLt k n)
+        case isTrue h =>
+          exact h
+        case isFalse h' =>
+          rewrite [Nat.not_lt_eq k n] at h'
+          have : k ≤ n := Nat.le_of_lt_succ p
+          have : k = n := Nat.le_antisymm this h'
+          contradiction
+      have : p_g ⟨k, p⟩ = p_g' ⟨k, p'⟩ := by dsimp
+      rewrite [this]
+      exact n_ih ⟨k, p'⟩
+
+-- -- 0 :: v.toList ++ List.zeros (offset_comp m p_g p_f - m) ++ List.zeros m ++ List.zeros n
+
+-- -- Store X i
+def execution_from_state_comp_store_succ_m_inputs (m : Nat) (p_g : Fin n → Program) (p_f : Program) (v : VectNat (m + 1)) :
+    execution_from_state (0 :: v.toList ++ List.zeros (offset_comp (m + 1) p_g p_f - (m + 1)) ++ List.zeros (m + 1) ++ List.zeros n)
+    (store_X_1_to_X_succ_n (offset_comp (m + 1) p_g p_f + 1) m)
+      = 0 :: v.toList ++ List.zeros (offset_comp (m + 1) p_g p_f - (m + 1)) ++ v.toList ++ List.zeros n := by
+  sorry
+
+def compute_store_g_i (p_g : Fin n → Program) (offset_store : Nat) (i : Fin n) : Program :=
+  p_g i ++ (X (offset_store + 1 + i) += X 0) ++ CLEAR X 0
+
+-- TODO: verify
+def compute_store_all_succ_n_g (n m : Nat) (p_g : Fin (n + 1) → Program) (p_f : Program) (offset_store : Nat) : Program :=
+  match n with
+  | 0 => compute_store_g_i p_g offset_store 0
+  | n + 1 => compute_store_g_i p_g offset_store 0 ++ compute_store_all_succ_n_g n m (fun i => p_g i.succ) p_f offset_store
+
+def execution_from_state_comp_compute_store_succ_n_g (m : Nat) (g : Fin (n + 1) → VectNat m → Nat) (p_g : Fin (n + 1) → Program)
+    (p_f : Program) (v : VectNat m) :
+    execution_from_state (0 :: v.toList ++ List.zeros (offset_comp m p_g p_f - m) ++ v.toList ++ List.zeros (n + 1))
+    (compute_store_all_succ_n_g n m p_g p_f (offset_comp m p_g p_f + m))
+      = 0 :: v.toList ++ List.zeros (offset_comp m p_g p_f - m) ++ v.toList ++ (Vector.ofFn (fun i => g i v)).toList := by
+  sorry
+
+def execution_from_state_comp_clear_succ_m_inputs (m : Nat) (p_g : Fin n → Program) (p_f : Program) (v : VectNat (m + 1)) :
+    execution_from_state (0 :: v.toList ++ List.zeros (offset_comp (m + 1) p_g p_f - (m + 1)) ++ v.toList ++ xs)
+      (clear_X_j_to_X_n_plus_j 1 m)
+        = 0 :: List.zeros (offset_comp (m + 1) p_g p_f) ++ v.toList ++ xs := by
+  sorry
+
+def execution_from_state_comp_setup_succ_n_inputs (m : Nat) (g : Fin (n + 1) → VectNat m → Nat) (p_g : Fin (n + 1) → Program)
+    (p_f : Program) (v : VectNat m) :
+    execution_from_state (0 :: List.zeros (offset_comp m p_g p_f) ++ v.toList ++ (Vector.ofFn (fun i => g i v)).toList)
+    (setup_X_j_to_X_n_plus_j (offset_comp m p_g p_f + m) 1 n)
+      = 0 :: (Vector.ofFn (fun i => g i v)).toList ++ List.zeros (offset_comp m p_g p_f - (n + 1)) ++ v.toList ++ (Vector.ofFn (fun i => g i v)).toList := by
+  sorry
+
+def execution_from_state_comp_clear_succ_n_z (m : Nat) (g : Fin (n + 1) → VectNat m → Nat) (p_g : Fin (n + 1) → Program)
+    (p_f : Program) (v : VectNat m) :
+    execution_from_state (0 :: (Vector.ofFn (fun i => g i v)).toList ++ List.zeros (offset_comp m p_g p_f - (n + 1)) ++ v.toList ++ (Vector.ofFn (fun i => g i v)).toList)
+    (clear_Z_0_to_Z_n (offset_comp m p_g p_f + m + 1) n)
+      = 0 :: (Vector.ofFn (fun i => g i v)).toList ++ List.zeros (offset_comp m p_g p_f - (n + 1)) ++ v.toList ++ List.zeros (n + 1) := by
+  sorry
+
+def execution_from_state_comp_execute_p_f (g : Fin (n + 1) → VectNat m → Nat) (p_g : Fin (n + 1) → Program)
+    (f_h : cleanly_computes p_f f) :
+    execution_from_state (0 :: (Vector.ofFn (fun i => g i v)).toList ++ List.zeros (offset_comp m p_g p_f - n) ++ v.toList ++ List.zeros n)
+      p_f =  f (Vector.ofFn (fun i => g i v)) :: (Vector.ofFn (fun i => g i v)).toList ++ List.zeros (offset_comp m p_g p_f - n) ++ v.toList ++ List.zeros n := by
+  sorry
+
+def execution_from_state_comp_clear_succ_n_inputs (m : Nat) (g : Fin (n + 1) → VectNat m → Nat) (p_g : Fin (n + 1) → Program)
+    (p_f : Program) (v : VectNat m) :
+    execution_from_state (x :: (Vector.ofFn (fun i => g i v)).toList ++ List.zeros (offset_comp m p_g p_f - (n + 1)) ++ v.toList ++ List.zeros (n + 1))
+    (clear_X_j_to_X_n_plus_j 1 n)
+      = x :: List.zeros (offset_comp m p_g p_f) ++ v.toList ++ List.zeros (n + 1) := by
+  sorry
+
+def execution_from_state_comp_setup_succ_m_inputs (m : Nat) (p_g : Fin n → Program) (p_f : Program) (v : VectNat (m + 1)) :
+    execution_from_state (x :: List.zeros (offset_comp (m + 1) p_g p_f) ++ v.toList ++ List.zeros n)
+    (setup_X_j_to_X_n_plus_j (offset_comp (m + 1) p_g p_f) 1 m)
+      = x :: v.toList ++ List.zeros (offset_comp (m + 1) p_g p_f - (m + 1)) ++ v.toList ++ List.zeros n := by
+  sorry
+
+def execution_from_state_comp_clear_succ_m_z (m : Nat) (p_g : Fin (n + 1) → Program) (p_f : Program) (v : VectNat m) :
+    execution_from_state (x :: v.toList ++ List.zeros (offset_comp m p_g p_f - m) ++ v.toList ++ List.zeros (n + 1))
+    (clear_Z_0_to_Z_n (offset_comp m p_g p_f + 1) m)
+      = x :: v.toList ++ List.zeros (offset_comp m p_g p_f - m) ++ List.zeros ((n + 1) + m) := by
+  sorry
+
+-- TODO: check if m = 0 is needed
+-- This was hard
+def comp_program (g : Fin n → VectNat m → Nat) (_ : cleanly_computes p_f f) (p_g : Fin n → Program)
+    (_ : ∀ i, cleanly_computes (p_g i) (g i)) : Program := match n with
+  | 0 => match m with
+    | 0 => p_f
+    | m + 1 =>
+         store_X_1_to_X_succ_n (offset_comp (m + 1) p_g p_f + 1) m
+      ++ clear_X_j_to_X_n_plus_j 1 m
+      ++ p_f
+      ++ setup_X_j_to_X_n_plus_j (offset_comp (m + 1) p_g p_f) 1 m
+      ++ clear_Z_0_to_Z_n (offset_comp m p_g p_f + 1) m
+  | n + 1 => match m with
+    | 0 =>
+         compute_store_all_succ_n_g n m p_g p_f (offset_comp m p_g p_f + m)
+      ++ setup_X_j_to_X_n_plus_j (offset_comp m p_g p_f + m) 1 n
+      ++ clear_Z_0_to_Z_n (offset_comp m p_g p_f + m + 1) n
+      ++ p_f
+      ++ clear_X_j_to_X_n_plus_j 1 n
+    | m + 1 =>
+         store_X_1_to_X_succ_n (offset_comp (m + 1) p_g p_f + 1) m
+      ++ compute_store_all_succ_n_g n m p_g p_f (offset_comp m p_g p_f + m)
+      ++ clear_X_j_to_X_n_plus_j 1 m
+      ++ setup_X_j_to_X_n_plus_j (offset_comp m p_g p_f + m) 1 n
+      ++ clear_Z_0_to_Z_n (offset_comp m p_g p_f + m + 1) n
+      ++ p_f
+      ++ clear_X_j_to_X_n_plus_j 1 n
+      ++ setup_X_j_to_X_n_plus_j (offset_comp (m + 1) p_g p_f) 1 m
+      ++ clear_Z_0_to_Z_n (offset_comp m p_g p_f + 1) m
+
+
+-- 1. def execution_from_state_comp_store_succ_m_inputs
+-- 2. def execution_from_state_comp_compute_store_succ_n_g
+-- 3. def execution_from_state_comp_clear_succ_m_inputs
+-- 4. def execution_from_state_comp_setup_succ_n_inputs
+-- 5. def execution_from_state_comp_clear_succ_n_z
+-- 6. def execution_from_state_comp_execute_p_f
+-- 7. def execution_from_state_comp_clear_succ_n_inputs
+-- 8. def execution_from_state_comp_setup_succ_m_inputs
+-- def execution_from_state_comp_clear_succ_m_z
+
+-- theorem comp_is_loop_computable_cleanly (g : Fin n → VectNat m → Nat) :
+--       loop_computable_cleanly f
+--     → (∀ i, loop_computable_cleanly (g i))
+--     → loop_computable_cleanly fun a => f (Vector.ofFn fun i => g i a) := by
+--   intro ⟨p_f, f_h⟩ g_h
+--   have ⟨p_g, g_h⟩ := forall_exists_function g g_h
+
+  -- sorry
+
+end comp_is_loop_computable_cleanly_proof
+
 
 /-
 theorem primrec_is_loop_computable_cleanly : Nat.Primrec' f → loop_computable_cleanly f := by
